Initial work to fix SameValue algorithm.
Uncomment existing code for algorithm and prove its decidability.

This code results in "AXIOM NOT REALIZED" errors when trying to run the
interpreter.
The new axioms the extraction process complains about are:
* prop_decidable
* same_value_dec

I'm now out of my depth and not sure how to continue this fix.
(See Issue #18)

coq/JsCommon.v
@@ -106,34 +106,27 @@ Definition type_of v :=
   | value_object _ => type_object
   end.
 
-(** LATER: Definition of the "SameValue" algorithm, which appears to
-    be equivalent to logical equality. The spec states:
-
-    Definition value_same v1 v2 :=
-      let ty1 := type_of v1 in
-      let ty2 := type_of v2 in
-      ifb ty1 <> ty2 then False else
-      match ty1 with
-      | type_undef => True
-      | type_null => True
-      | type_number =>
-          ifb   v1 = (prim_number JsNumber.nan)
-             /\ v2 = (prim_number JsNumber.nan) then True
-          else ifb    v1 = (prim_number JsNumber.zero)
-                  /\ v2 = (prim_number JsNumber.neg_zero) then False
-          else ifb    v1 = (prim_number JsNumber.neg_zero)
-                  /\ v2 = (prim_number JsNumber.zero) then False
-          else (v1 = v2)
-      | type_string => (v1 = v2)
-      | type_bool => (v1 = v2)
-      | type_object => (v1 = v2)
-      end.
-
-    Which is equivalent to:
-*)
-(* LATER: problem of the several representations of NaN *)
-
-Definition same_value v1 v2 := (v1 = v2).
+(** Specification method SameValue used internally by [[DefineOwnProperty]] (9.12) *)
+Definition same_value v1 v2 :=
+  let ty1 := type_of v1 in
+  let ty2 := type_of v2 in
+  ifb ty1 <> ty2 then False else
+  match ty1 with
+  | type_undef => True
+  | type_null => True
+  | type_number =>
+      ifb   v1 = (prim_number JsNumber.nan)
+         /\ v2 = (prim_number JsNumber.nan) then True
+      else ifb    v1 = (prim_number JsNumber.zero)
+              /\ v2 = (prim_number JsNumber.neg_zero) then False
+      else ifb    v1 = (prim_number JsNumber.neg_zero)
+              /\ v2 = (prim_number JsNumber.zero) then False
+      else (v1 = v2)
+  | type_string => (v1 = v2)
+  | type_bool => (v1 = v2)
+  | type_object => (v1 = v2)
+  end.
+(* LATER: check problem of the several representations of NaN *)
 
 (**************************************************************)
 (** ** Operations on event lists *)
