coq/JsCommonAux.v
@@ -59,10 +59,12 @@ Proof.
   destruct x; destruct y; simpls~; typeclass.
 Qed.
 
-Lemma if_some_value_then_same_self : forall vo,
-  if_some_value_then_same vo vo.
+Global Instance same_value_dec : forall v1 v2,
+  Decidable (same_value v1 v2).
 Proof.
-  introv. unfolds. unfolds. destruct~ vo. reflexivity.
+  introv. unfold same_value. case_if.
+  apply prop_decidable.
+  apply prop_decidable.
 Qed.
 
 Lemma if_some_bool_then_same_self : forall bo,
